code/ecdsap256sha2/Hacl.Impl.P256.DH.fst
@@ -41,10 +41,22 @@ let ecp256dh_i result scalar =
     secretToPublic resultBuffer scalar tempBuffer; 
     let flag = isPointAtInfinityPrivate resultBuffer in 
   let h2 = ST.get() in
+    changeEndian resultBufferX;
+    changeEndian resultBufferY;
+    
     toUint8 resultBufferX resultX;
-      lemma_core_1 resultBufferX h2;
-      lemma_core_1 resultBufferY h2;
     toUint8 resultBufferY resultY;
+  
+  let h3 = ST.get() in 
+  
+  lemma_core_0 resultBufferX h2;
+  lemma_nat_from_to_intseq_le_preserves_value 4 (as_seq h2 resultBufferX);
+  Hacl.Spec.ECDSA.changeEndianLemmaFromBeToLe (as_nat h2 resultBufferX) h3 resultX;
+
+  lemma_core_0 resultBufferY h2;
+  lemma_nat_from_to_intseq_le_preserves_value 4 (as_seq h2 resultBufferY);
+  Hacl.Spec.ECDSA.changeEndianLemmaFromBeToLe (as_nat h2 resultBufferY) h3 resultY;
+  
   pop_frame(); 
     flag
 
@@ -65,8 +77,10 @@ val _ecp256dh_r: result: lbuffer uint64 (size 12) -> pubKey: lbuffer uint64 (siz
 	if not (verifyQValidCurvePointSpec (pointJacX, pointJacY, pointJacZ)) then 
 	  uint_v r = maxint U64
 	else 
-	  let xN, yN, zN = scalar_multiplication (as_seq h0 scalar) (pointJacX, pointJacY, pointJacZ) in 
-	  xN == x3 /\ yN == y3 /\ zN == z3 /\
+	  x3 < prime256 /\ y3 < prime256 /\ z3 < prime256 /\ 
+	  (
+	    let xN, yN, zN = scalar_multiplication (as_seq h0 scalar) (pointJacX, pointJacY, pointJacZ) in 
+	    xN == x3 /\ yN == y3 /\ zN == z3 /\
 	  (
 	    if isPointAtInfinity (xN, yN, zN) then 
 	      uint_v r = maxint U64
@@ -75,6 +89,9 @@ val _ecp256dh_r: result: lbuffer uint64 (size 12) -> pubKey: lbuffer uint64 (siz
 	  )
       )
   )
+
+)
+
 
 let _ecp256dh_r result pubKey scalar = 
   push_frame();
@@ -113,20 +130,35 @@ let ecp256dh_r result pubKey scalar =
 	let pubKeyX = sub pubKey (size 0) (size 32) in 
 	let pubKeyY = sub pubKey (size 32) (size 32) in 
 
-      toUint64 pubKeyX publicKeyFelemX;
-      toUint64 pubKeyY publicKeyFelemY;
+      toUint64ChangeEndian pubKeyX publicKeyFelemX;
+      toUint64ChangeEndian pubKeyY publicKeyFelemY;
       
       let h1 = ST.get() in 
-	lemma_core_0 publicKeyFelemX h1;
-	Lib.ByteSequence.uints_from_bytes_le_nat_lemma #U64 #SEC #4 (as_seq h1 pubKeyX);
-	lemma_core_0 publicKeyFelemY h1;
-	Lib.ByteSequence.uints_from_bytes_le_nat_lemma #U64 #SEC #4 (as_seq h1 pubKeyY); 
+      lemma_core_0 publicKeyFelemX h1;
+      Hacl.Spec.ECDSA.changeEndianLemma (uints_from_bytes_be (as_seq h0 pubKeyX));
+      uints_from_bytes_be_nat_lemma #U64 #_ #4 (as_seq h1 pubKeyX);   
+
+      lemma_core_0 publicKeyFelemY h1;
+      Hacl.Spec.ECDSA.changeEndianLemma (uints_from_bytes_be (as_seq h0 pubKeyY));
+      uints_from_bytes_be_nat_lemma #U64 #_ #4 (as_seq h1 pubKeyY);  
 	
 	let flag = _ecp256dh_r resultBufferFelem publicKeyAsFelem scalar in 
       let h2 = ST.get() in 	
+
+      changeEndian resultBufferFelemX;
+      changeEndian resultBufferFelemY;
       toUint8 resultBufferFelemX resultX;
-	lemma_core_1 resultBufferFelemX h2;
       toUint8 resultBufferFelemY resultY;
-	lemma_core_1 resultBufferFelemY h2;
+
+      let h3 = ST.get() in 
+      
+      lemma_core_0 resultBufferFelemX h2;
+      lemma_nat_from_to_intseq_le_preserves_value 4 (as_seq h2 resultBufferFelemX);
+      Hacl.Spec.ECDSA.changeEndianLemmaFromBeToLe (as_nat h2 resultBufferFelemX) h3 resultX;
+
+      lemma_core_0 resultBufferFelemY h2;
+      lemma_nat_from_to_intseq_le_preserves_value 4 (as_seq h2 resultBufferFelemY);
+      Hacl.Spec.ECDSA.changeEndianLemmaFromBeToLe (as_nat h2 resultBufferFelemY) h3 resultY;
+    
       pop_frame();
       flag
