code/ecdsap256sha2/Hacl.Impl.P256.DH.fsti
@@ -25,6 +25,7 @@ open Hacl.Impl.LowLevel
 open Hacl.Impl.P256
 open Hacl.Impl.P256.Signature.Common
 
+
 val ecp256dh_i: result: lbuffer uint8 (size 64) -> scalar: lbuffer uint8 (size 32) -> Stack uint64
   (requires fun h -> live h result /\ live h scalar /\ disjoint result scalar /\
     Lib.ByteSequence.nat_from_bytes_le (as_seq h scalar) >= 1 /\
@@ -36,8 +37,8 @@ val ecp256dh_i: result: lbuffer uint8 (size 64) -> scalar: lbuffer uint8 (size 3
       let resultX = gsub result (size 0) (size 32) in 
       let resultY = gsub result (size 32) (size 32) in 
       if isPointAtInfinity (xN, yN, zN) then uint_v r = maxint U64 else uint_v r = 0 /\
-      Lib.ByteSequence.nat_from_bytes_le (as_seq h1 resultX) == xN /\
-      Lib.ByteSequence.nat_from_bytes_le (as_seq h1 resultY) == yN
+      as_seq h1 resultX == nat_to_bytes_be 32 xN /\
+      as_seq h1 resultY == nat_to_bytes_be 32 yN 
     )  
   )
 
@@ -53,15 +54,15 @@ val ecp256dh_r: result: lbuffer uint8 (size 64) -> pubKey: lbuffer uint8 (size 6
       modifies (loc result) h0 h1 /\ 
 	(
 	  let pubKeyX, pubKeyY = gsub pubKey (size 0) (size 32), gsub pubKey (size 32) (size 32) in 
-	  let x, y = nat_from_bytes_le (as_seq h0 pubKeyX), nat_from_bytes_le (as_seq h0 pubKeyY) in 
+	  let x, y = nat_from_bytes_be (as_seq h0 pubKeyX), nat_from_bytes_be (as_seq h0 pubKeyY) in 
 	  let resultX, resultY = gsub result (size 0) (size 32), gsub result (size 32) (size 32) in 
-	  let x3, y3 = nat_from_bytes_le (as_seq h1 resultX), nat_from_bytes_le (as_seq h1 resultY) in 
 	  let pointJacX, pointJacY, pointJacZ = toJacobianCoordinates (x, y) in 
 	  if not (verifyQValidCurvePointSpec (pointJacX, pointJacY, pointJacZ)) then 
 	    uint_v flag = maxint U64
 	  else 
 	    let xN, yN, zN = scalar_multiplication (as_seq h0 scalar) (pointJacX, pointJacY, pointJacZ) in 
-	    xN == x3 /\ yN == y3 /\
+	    as_seq h1 resultX == nat_to_bytes_be 32 xN /\
+	    as_seq h1 resultY == nat_to_bytes_be 32 yN /\
 	    (
 	      if isPointAtInfinity (xN, yN, zN) then 
 		uint_v flag = maxint U64
