specs/ecdsap256sha2/Hacl.Spec.P256.Normalisation.fst
@@ -15,11 +15,12 @@ let prime = prime256
 
 open FStar.Mul  
 #reset-options " --z3rlimit 300" 
-val lemma_norm_as_specification: xD: nat -> yD: nat -> zD: nat -> 
+val lemma_norm_as_specification: xD: nat{xD < prime256} -> yD: nat{yD < prime256} -> zD: nat {zD < prime256} -> 
   x3 : nat {x3 == xD * (pow (zD * zD) (prime-2) % prime) % prime}-> 
   y3 : nat {y3 == yD * (pow (zD * zD * zD) (prime -2) % prime) % prime} -> 
   z3: nat {if isPointAtInfinity(xD, yD, zD) then z3 == 0 else z3 == 1} -> 
-    Lemma (let (xN, yN, zN) = _norm (xD, yD, zD) in 
+  Lemma (
+  let (xN, yN, zN) = _norm (xD, yD, zD) in 
   x3 == xN /\ y3 == yN /\ z3 == zN)
 
 
